Split to multiple files

src/ocamlmm/OCamlToimm_s_prog.v
@@ -1,7 +1,6 @@
 (******************************************************************************)
 (** * ocaml MM is weaker than IMM_S   *)
 (******************************************************************************)
-Require Import Classical Peano_dec.
 From hahn Require Import Hahn.
 Require Import Omega.
 Require Import Events.
@@ -10,26 +9,18 @@ Require Import Execution_eco.
 Require Import imm_common.
 Require Import imm_s_hb.
 Require Import imm_s.
-Require Import OCaml.
-Require Import OCamlToimm_s. 
 Require Import Prog.
 Require Import ProgToExecution.
 Require Import ProgToExecutionProperties.
 From PromisingLib Require Import Basic Loc.
 Require Import Basics. 
 Set Implicit Arguments.
-Remove Hints plus_n_O.
-
-
-Variable exchange_reg: Reg.t.
-Lemma exchange_reg_dedicated: True.
-Proof. Admitted. 
 
 
 Section OCaml_Program.
 
   Inductive Oistep_ tid labels s1 s2 instr dindex (GT0: dindex > 0): Prop :=
-  | assign reg expr
+  | Oassign reg expr
            (LABELS : labels = nil)
            (II : instr = Instr.assign reg expr)
            (UPC : s2.(pc) = s1.(pc) + 1)
@@ -38,7 +29,7 @@ Section OCaml_Program.
            (UREGS : s2.(regf) = RegFun.add reg (RegFile.eval_expr s1.(regf) expr) s1.(regf))
            (UDEPS : s2.(depf) = RegFun.add reg (DepsFile.expr_deps s1.(depf) expr) s1.(depf))
            (UECTRL : s2.(ectrl) = s1.(ectrl))
-  | if_ expr shift
+  | Oif_ expr shift
         (LABELS : labels = nil)
         (II : instr = Instr.ifgoto expr shift)
         (UPC   : if Const.eq_dec (RegFile.eval_expr s1.(regf) expr) 0
@@ -49,7 +40,7 @@ Section OCaml_Program.
         (UREGS : s2.(regf) = s1.(regf))
         (UDEPS : s2.(depf) = s1.(depf))
         (UECTRL : s2.(ectrl) = (DepsFile.expr_deps s1.(depf) expr) ∪₁ s1.(ectrl))
-  | load ord reg lexpr val l
+  | Oload ord reg lexpr val l
          (L: l = RegFile.eval_lexpr s1.(regf) lexpr)
          (II : instr = Instr.load ord reg lexpr)
          (LABELS : labels = [Aload false ord (RegFile.eval_lexpr s1.(regf) lexpr) val])
@@ -61,7 +52,7 @@ Section OCaml_Program.
          (UREGS : s2.(regf) = RegFun.add reg val s1.(regf))
          (UDEPS : s2.(depf) = RegFun.add reg (eq (ThreadEvent tid s1.(eindex))) s1.(depf))
          (UECTRL : s2.(ectrl) = s1.(ectrl))
-  | store ord lexpr expr l v x
+  | Ostore ord lexpr expr l v x
           (L: l = RegFile.eval_lexpr s1.(regf) lexpr)
           (V: v = RegFile.eval_expr  s1.(regf)  expr)
           (X: x = Xpln)
@@ -76,7 +67,7 @@ Section OCaml_Program.
           (UREGS : s2.(regf) = s1.(regf))
           (UDEPS : s2.(depf) = s1.(depf))
           (UECTRL : s2.(ectrl) = s1.(ectrl))
-  | fence ord 
+  | Ofence ord 
           (LABELS : labels = [Afence ord])
           (II : instr = Instr.fence ord)
           (UPC   : s2.(pc) = s1.(pc) + 1)
@@ -85,7 +76,7 @@ Section OCaml_Program.
           (UREGS : s2.(regf) = s1.(regf))
           (UDEPS : s2.(depf) = s1.(depf))
           (UECTRL : s2.(ectrl) = s1.(ectrl))
-  | cas_un expr_old expr_new xmod ordr ordw reg lexpr val l
+  | Ocas_un expr_old expr_new xmod ordr ordw reg lexpr val l
            (L: l = RegFile.eval_lexpr s1.(regf) lexpr)
            (NEXPECTED : val <> RegFile.eval_expr s1.(regf) expr_old)
            (LABELS : labels = [Aload true ordr l val])
@@ -99,7 +90,7 @@ Section OCaml_Program.
            (UREGS : s2.(regf) = RegFun.add reg val s1.(regf))
            (UDEPS : s2.(depf) = RegFun.add reg (eq (ThreadEvent tid s1.(eindex))) s1.(depf))
            (UECTRL : s2.(ectrl) = s1.(ectrl))
-  | cas_suc expr_old expr_new xmod ordr ordw reg lexpr l expected new_value
+  | Ocas_suc expr_old expr_new xmod ordr ordw reg lexpr l expected new_value
             (L: l = RegFile.eval_lexpr s1.(regf) lexpr)
             (EXPECTED: expected = RegFile.eval_expr s1.(regf) expr_old)
             (NEW: new_value = RegFile.eval_expr s1.(regf) expr_new)
@@ -116,7 +107,7 @@ Section OCaml_Program.
             (UREGS : s2.(regf) = RegFun.add reg expected s1.(regf))
             (UDEPS : s2.(depf) = RegFun.add reg (eq (ThreadEvent tid s1.(eindex))) s1.(depf))
             (UECTRL : s2.(ectrl) = s1.(ectrl))
-  | inc expr_add xmod ordr ordw reg lexpr val l nval
+  | Oinc expr_add xmod ordr ordw reg lexpr val l nval
         (L: l = RegFile.eval_lexpr s1.(regf) lexpr)
         (NVAL: nval = val + RegFile.eval_expr s1.(regf) expr_add)
         (LABELS : labels = [Astore xmod ordw l nval; Aload true ordr l val])
@@ -133,7 +124,7 @@ Section OCaml_Program.
         (UREGS : s2.(regf) = RegFun.add reg val s1.(regf))
         (UDEPS : s2.(depf) = RegFun.add reg (eq (ThreadEvent tid s1.(eindex))) s1.(depf))
         (UECTRL : s2.(ectrl) = s1.(ectrl))
-  | exchange new_expr xmod ordr ordw reg loc_expr old_value loc new_value
+  | Oexchange new_expr xmod ordr ordw reg loc_expr old_value loc new_value
              (L: loc = RegFile.eval_lexpr s1.(regf) loc_expr)
              (NVAL: new_value = RegFile.eval_expr s1.(regf) new_expr)
              (LABELS : labels = [Astore xmod ordw loc new_value;
@@ -159,21 +150,21 @@ Section OCaml_Program.
     ⟪ ISTEP: exists instr dindex', 
         Some instr = List.nth_error s1.(instrs) s1.(pc) /\
         @Oistep_ tid labels s1 s2 instr (S dindex') (gt_Sn_O dindex')⟫.
-
+  
   Definition Ostep (tid : thread_id) s1 s2 :=
     exists lbls, Oistep tid lbls s1 s2.
 
   Definition is_ocaml_mode mode :=
     match mode with
-    | Orlx | Osc => True
-    | _ => False
+    | Orlx | Osc => true
+    | _ => false
     end. 
   
   Definition is_ocaml_instruction instr :=
     match instr with
-    | Instr.assign _ _ | Instr.ifgoto _ _ => True
+    | Instr.assign _ _ | Instr.ifgoto _ _ => true
     | Instr.load mode _ _ | Instr.store mode _ _ => is_ocaml_mode mode
-    | _ => False
+    | _ => false
     end. 
 
   Definition Othread_execution (tid : thread_id) (insts : list Prog.Instr.t) (pe : execution) :=
@@ -182,7 +173,42 @@ Section OCaml_Program.
       ⟪ TERMINAL : is_terminal s ⟫ /\
       ⟪ PEQ : s.(G) = pe ⟫.
 
-  Definition OCamlProgram (prog: Prog.Prog.t) := True. 
+  (* separation should be consistent across all threads *)
+ 
+  (* Definition is_matching_mode instr mode := *)
+  (*   match instr with *)
+  (*   | Instr.load md _ _ | Instr.store md _ _ => (mode = md) *)
+  (*   | _ => True *)
+  (*   end. *)
+
+  Definition instr_mode instr :=
+    match instr with
+    | Instr.load mode _ _ | Instr.store mode _ _ | Instr.fence mode => Some mode
+    | Instr.update _ _ mode_r mode_w _ _ => Some mode_r (* assume that mode_r = mode_w *)
+    | _ => None
+    end. 
+
+  Definition instr_locs instr :=
+    match instr with
+    | Instr.load _ _ lxpr | Instr.store _ lxpr _
+    | Instr.update _ _ _ _ _ lxpr => match lxpr with
+                                  | Instr.lexpr_loc l => [l]
+                                  | Instr.lexpr_choice _ l1 l2 => [l1;  l2]
+                                  end
+    | _ => []
+    end. 
+
+  Definition locations_separated prog := forall (loc : Loc.t), exists mode,
+        is_ocaml_mode mode /\
+        (forall tid PO (INTHREAD: IdentMap.find tid prog = Some PO)
+           instr (INPROG: In instr PO)
+           (AT_LOC: In loc (instr_locs instr)),
+            Some mode = instr_mode instr). 
+
+  Definition OCamlProgram (prog: Prog.Prog.t) :=
+    (forall tid PO (INTHREAD: IdentMap.find tid prog = Some PO),
+        forallb is_ocaml_instruction PO) /\
+    locations_separated prog. 
 
   Definition Oprogram_execution prog (OPROG: OCamlProgram prog) (G : execution) :=
     (forall e (IN: G.(acts_set) e), is_init e \/ IdentMap.In (tid e) prog)
@@ -191,559 +217,3 @@ Section OCaml_Program.
             /\ thread_restricted_execution G thread pe.
   
 End OCaml_Program.
-
-
-Section OCaml_IMM_Compilation.
-
-  Inductive is_instruction_compiled : Prog.Instr.t -> list Prog.Instr.t -> Prop :=
-  | compiled_Rna_alt lhs loc:
-      let ld := (Instr.load Orlx lhs loc) in
-      is_instruction_compiled (ld) ([ld])
-  | compiled_Wna_alt loc val:
-      let st := (Instr.store Orlx loc val) in
-      let f := (Instr.fence Oacqrel) in
-      is_instruction_compiled (st) ([f; st])
-  | compiled_Rat_alt lhs loc:
-      let ld := (Instr.load Osc lhs loc) in
-      let f := (Instr.fence Oacq) in
-      is_instruction_compiled (ld) ([f; ld])
-  | compiled_Wat_alt loc val:
-      let st := (Instr.store Osc loc val) in
-      let exc := (Instr.update (Instr.exchange val) Xpln Osc Osc exchange_reg loc) in
-      let f := (Instr.fence Oacq) in
-      is_instruction_compiled (st) ([f; exc])
-  | compiled_assign_alt lhs rhs:
-      let asn := (Instr.assign lhs rhs) in
-      is_instruction_compiled (asn) ([asn])
-  | compiled_ifgoto_alt e n:
-      let igt := (Instr.ifgoto e n) in
-      is_instruction_compiled (igt) ([igt]).
-  
-  Inductive is_thread_compiled_alt : list Prog.Instr.t -> list Prog.Instr.t -> Prop :=
-  | compiled_empty_alt: is_thread_compiled_alt [] []
-  | compiled_add_alt oinstr block ro ri
-                     (instr_compiled: is_instruction_compiled oinstr block)
-                     (rest: is_thread_compiled_alt ro ri):
-      is_thread_compiled_alt (ro ++ [oinstr]) (ri ++ block).
-
-  Definition is_compiled (po: Prog.Prog.t) (pi: Prog.Prog.t) :=
-    ⟪ SAME_THREADS: forall t_id, IdentMap.In t_id po <-> IdentMap.In t_id pi ⟫ /\
-    forall thread to ti (TO: IdentMap.find thread po = Some to)
-      (TI: IdentMap.find thread pi = Some ti), is_thread_compiled_alt to ti.
-
-End OCaml_IMM_Compilation.   
-
-Section SEQ_STEPS.
-  
-  Inductive step_seq : thread_id -> list ((list label)*Prog.Instr.t) -> state -> state -> Prop :=
-  | empty_step_seq tid st: step_seq tid [] st st
-  | next_step_seq
-      tid labels insn cur_st next_st fin_st
-      (STEP: istep_ tid labels cur_st next_st insn)
-      rest (REST: step_seq tid rest next_st fin_st):
-      step_seq tid ((labels,insn)::rest) cur_st fin_st.
-
-  Definition sublist {A: Type} (l: list A) (start len: nat) : list A.
-  Admitted.
-  
-  Definition oseq_istep tid (labels_blocks: list (list label)) sti1 sti2 :=
-    let n_steps := length labels_blocks in
-    let block := sublist (instrs sti1) (pc sti1) n_steps in
-    ⟪ INSTRS : sti1.(instrs) = sti2.(instrs) ⟫ /\
-    ⟪ ISTEP: exists labelsblocks_insns,
-        labelsblocks_insns = List.combine labels_blocks block /\
-        step_seq tid labelsblocks_insns sti1 sti2 ⟫ /\
-    ⟪ COMPILED_BLOCK: exists oinstr, is_instruction_compiled oinstr block ⟫.
-  
-  Definition oseq_step (tid : thread_id) sti1 sti2 :=
-    exists labels_blocks, oseq_istep tid labels_blocks sti1 sti2.
-  
-End SEQ_STEPS. 
-  
-Section ClosuresProperties.
-  Variable A: Type.
-  Variable r: relation A. 
-  
-  Lemma steps_split n a b (SPLIT: a + b = n) x y:
-    r^^n x y <-> exists z, r^^a x z /\ r^^b z y.
-  Proof.
-    split. 
-    { ins.
-      pose proof (pow_nm a b r) as STEPS_SPLIT.
-      pose proof (same_relation_exp STEPS_SPLIT x y).
-      rewrite SPLIT in H0. apply H0 in H. destruct H as [z STEPSz ].
-      eauto. }
-    ins. desf.
-    pose proof (pow_nm a b r) as STEPS_SPLIT.
-    pose proof (same_relation_exp STEPS_SPLIT x y).
-    apply H1. red. exists z. auto.     
-  Qed. 
-  
-  Lemma steps_sub n x y m (LEQ: m <= n): r^^n x y -> exists z, r^^m x z. 
-  Proof.
-    ins.
-    pose proof (pow_nm m (n-m) r) as STEPS_SPLIT.
-    pose proof (same_relation_exp STEPS_SPLIT x y).
-    rewrite Const.add_sub_assoc in H0; [| auto]. rewrite minus_plus in H0.
-    apply H0 in H. destruct H as [z STEPSz]. desc. 
-    eauto. 
-  Qed.
-
-  Lemma steps0 x y: r^^0 x y <-> x = y.
-  Proof. simpl. split; basic_solver. Qed.
-  
-  Lemma steps_indices n x y:
-    r^^n x y -> forall i (INDEX: i < n), exists z1 z2, r^^i x z1 /\ r z1 z2.
-  Proof.
-    intros Rn i LT. 
-    assert (LEQ: i + 1 <= n) by omega. 
-    pose proof (steps_sub x y LEQ Rn) as [z2 Ri1].
-    pose proof (@steps_split (i+1) i 1 eq_refl x z2).
-    apply H in Ri1. destruct Ri1 as [z1 [Ri R1]].
-    exists z1. exists z2. split; [auto| ]. 
-    apply (same_relation_exp (pow_unit r)). auto.
-  Qed. 
-  
-  Lemma step_prev x y k: r^^(S k) x y <-> exists z, r^^k x z /\ r z y.
-  Proof. ins. Qed.
-  
-  Lemma crt_num_steps a b: r＊ a b <-> exists n, r ^^ n a b.
-  Proof.
-    split.
-    { ins. rewrite clos_refl_transE in H. destruct H.
-      { exists 0. split; auto. }
-      induction H. 
-      { exists 1. simpl. basic_solver. }
-      destruct IHclos_trans1 as [n1 IH1]. destruct IHclos_trans2 as [n2 IH2]. 
-      exists (n1+n2). (* split; [omega | ]. *)
-      pose proof (@pow_nm _ n1 n2 r) as POW. destruct POW as [POW _].
-      specialize (POW x z). apply POW.
-      red. exists y. desc. split; auto. }
-    ins. destruct H as [n STEPS].
-    rewrite clos_refl_transE.
-    destruct n.
-    { left. desc.  simpl in STEPS. generalize STEPS. basic_solver 10. }
-    right. desc.
-    pose proof ctEE. specialize (H _ r). destruct H as [_ POW].
-    apply POW. basic_solver. 
-  Qed.
-
-End ClosuresProperties. 
-
-Section OCamlMM_TO_IMM_S_PROG.
-
-  Notation "'E' G" := G.(acts_set) (at level 1).
-  Notation "'R' G" := (fun a => is_true (is_r G.(lab) a)) (at level 1).
-  Notation "'W' G" := (fun a => is_true (is_w G.(lab) a)) (at level 1).
-  Notation "'RW' G" := (R G ∪₁ W G) (at level 1).
-  Notation "'F' G" := (fun a => is_true (is_f G.(lab) a)) (at level 1).
-  Notation "'ORlx' G" := (fun a => is_true (is_only_rlx G.(lab) a)) (at level 1).
-  Notation "'Sc' G" := (fun a => is_true (is_sc G.(lab) a)) (at level 1). 
-  Notation "'Acq' G" := (fun a => is_true (is_acq G.(lab) a)) (at level 1). 
-  Notation "'Acqrel' G" := (fun a => is_true (is_acqrel G.(lab) a)) (at level 1). 
-  Notation "'R_ex' G" := (fun a => is_true (R_ex G.(lab) a)) (at level 1).
-  Notation "'hbo'" := (OCaml.hb). 
-  Notation "'same_loc' G" := (same_loc G.(lab)) (at level 1).
-  Notation "'Tid_' t" := (fun x => tid x = t) (at level 1).
-    
-  Definition prepend_events (A: actid -> Prop) (shift: nat) := compose A (fun e => ThreadEvent (tid e) (index e + shift)).
-  Notation "f '∙' g" := (compose f g) (at level 1). (* default notation is for other scope*)  
-    
-  Definition same_behavior_local (GO GI: execution) :=
-    let Facq' := prepend_events (E GO ∩₁ Sc GO) 2 in
-    let Facqrel' := prepend_events (E GO ∩₁ W GO ∩₁ ORlx GO) 2 in
-    let R' := prepend_events (E GO ∩₁ W GO ∩₁ Sc GO) 1 in
-    
-    let rmw_pair r w := (tid r = tid w) /\ (index r = index w - 1) in
-    
-    let wf_labels :=
-        (GI.(lab) = GO.(lab)) /\
-        (forall e (FACQ: Facq' e), GI.(lab) e = Afence Oacq) /\
-        (forall e (FACQ: Facqrel' e), GI.(lab) e = Afence Oacqrel) /\
-        (forall e (R': R' e), exists loc val w,
-              GI.(lab) e = Aload true Osc loc val /\
-              GO.(lab) w = Astore Xpln Osc loc val /\
-              rmw_pair e w) in
-    ⟪ADD_EVENTS: E GI ≡₁ E GO ∪₁ Facq' ∪₁ Facqrel' ∪₁ R' ⟫ /\
-    ⟪EXT_LABELS: wf_labels ⟫ /\
-    ⟪NEW_RMW: GI.(rmw) ≡ fun r w => (E GI ∩₁ R GI ∩₁ Sc GI) r /\ (E GI ∩₁ W GI ∩₁ Sc GI) w /\ rmw_pair r w ⟫.
-
-  Definition same_behavior (GO GI: execution) :=
-    ⟪SAME_LOCAL: same_behavior_local GO GI ⟫ /\
-    ⟪SAME_CO: GI.(co) ≡ GO.(co)⟫ /\
-    ⟪EXT_RF: GO.(rf) ≡ GI.(rf) ⨾ ⦗set_compl (dom_rel GI.(rmw))⦘⟫.
-        
-  Definition prefix {A: Type} (p l: list A) :=
-    exists s, p ++ s = l.
-  
-  Definition prefix_option {A: Type} (p: list A) (lo: option (list A)):=
-    exists l s, lo = Some l /\ p ++ s = l.
-  
-  Record Wf_local (G: execution) :=
-    {  wf_index' : forall a b, 
-        (E G) a /\ (E G) b /\ a <> b /\ tid a = tid b /\ ~ is_init a -> index a <> index b;
-       wf_dataD' : G.(data) ≡ ⦗R G⦘ ⨾ G.(data) ⨾ ⦗W G⦘ ;
-       ctrl_sb' : G.(ctrl) ⨾ G.(sb) ⊆ G.(ctrl) ;
-       wf_addrD' : G.(addr) ≡ ⦗R G⦘ ⨾ G.(addr) ⨾ ⦗RW G⦘ ;
-       wf_ctrlD' : G.(ctrl) ≡ ⦗R G⦘ ⨾ G.(ctrl) ;
-       wf_rmwD' : G.(rmw) ≡ ⦗R_ex G⦘ ⨾ G.(rmw) ⨾ ⦗W G⦘ ;
-       wf_rmwl' : G.(rmw) ⊆ same_loc G ;
-       wf_rmwi' : G.(rmw) ⊆ immediate G.(sb) ;
-       wf_rmw_depD' : G.(rmw_dep) ≡ ⦗R G⦘ ⨾ G.(rmw_dep) ⨾ ⦗R_ex G⦘ ;
-    }. 
-  
-  Record Wf_global (G: execution) :=
-    {
-      data_in_sb' : G.(data) ⊆ G.(sb) ;
-      addr_in_sb' : G.(addr) ⊆ G.(sb) ;
-      ctrl_in_sb' : G.(ctrl) ⊆ G.(sb) ;
-      rmw_dep_in_sb' : G.(rmw_dep) ⊆ G.(sb) ;
-      wf_rfE' : G.(rf) ≡ ⦗E G⦘ ⨾ G.(rf) ⨾ ⦗E G⦘ ;
-      wf_rfD' : G.(rf) ≡ ⦗W G⦘ ⨾ G.(rf) ⨾ ⦗R G⦘ ;
-      wf_rfl' : G.(rf) ⊆ same_loc G;
-      wf_rfv' : funeq (val G.(lab)) G.(rf) ;
-      wf_rff' : functional G.(rf)⁻¹ ;
-      wf_coE' : G.(co) ≡ ⦗E G⦘ ⨾ G.(co) ⨾ ⦗E G⦘ ;
-      wf_coD' : G.(co) ≡ ⦗W G⦘ ⨾ G.(co) ⨾ ⦗W G⦘ ;
-      wf_col' : G.(co) ⊆ same_loc G;
-      co_trans' : transitive G.(co) ;
-      wf_co_total' : forall ol, is_total (E G ∩₁ W G ∩₁ (fun x => loc G.(lab) x = ol)) G.(co) ;
-      co_irr' : irreflexive G.(co) ;
-      wf_init' : forall l, (exists b, E G b /\ loc G.(lab) b = Some l) -> E G (InitEvent l) ;
-      wf_init_lab' : forall l, G.(lab) (InitEvent l) = Astore Xpln Opln l 0 ;       
-    }.
-      
-  Lemma compilation_same_length PO PI (COMP: is_thread_compiled_alt PO PI):
-    exists BPI, length PO = length BPI /\ flatten BPI = PI. 
-  Proof.
-    (* induction COMP. *)
-    (* { auto. } *)
-    (* all: do 2 rewrite app_length; rewrite IHCOMP; auto. *)
-    (* Qed. *)
-  Admitted. 
-
-  Definition mm_similar_states_alt (sto sti: state) :=
-    is_thread_compiled_alt sto.(instrs) sti.(instrs)  /\
-    is_thread_compiled_alt (firstn sto.(pc) sto.(instrs)) (firstn sti.(pc) sti.(instrs)) /\
-    same_behavior_local sto.(G) sti.(G) /\
-    sto.(regf) = sti.(regf) /\
-    sto.(eindex) = sti.(eindex). 
-  
-  (* Definition next_compilation_block sti (CORR: exists sto, mm_similar_states_alt sto sti) (NOT_END: pc sti < length (instrs sti)) : list Prog.Instr.t. *)
-  (* Admitted. *)
-  
-  Lemma pair_step_alt sto sti (MM_SIM: mm_similar_states_alt sto sti)
-        tid sti' (SEQ_STEP: oseq_step tid sti sti'):
-    exists sto', Ostep tid sto sto' /\ mm_similar_states_alt sto' sti'.
-  Proof. Admitted.
-  
-  Lemma first_end {A: Type} (l: list A) n x (NTH: Some x = List.nth_error l n):
-    firstn (n + 1) l = firstn n l ++ [x].
-  Proof.
-    ins. 
-    symmetry in NTH. apply nth_error_split in NTH as [l1 [l2 [CAT H]]].
-    rewrite <- H. pose proof (@firstn_app_2 A 1 l1 (x :: l2)).
-    rewrite CAT. simpl in H0. rewrite H0.
-    pose proof (@firstn_app_2 A 0 l1). simpl in H1. rewrite app_nil_r, NPeano.Nat.add_0_r in H1.
-    rewrite H1. auto. 
-  Qed. 
-    
-  Lemma group_steps k sti tid (REACH: (step tid) ^^ k (init (instrs sti)) sti)
-        (BY_GROUPS: exists PO, is_thread_compiled_alt PO (firstn k sti.(instrs))):
-    (oseq_step tid)＊ (init (instrs sti)) sti.
-  Proof. Admitted. 
-    
-  Lemma init_mm_same: forall PO PI (COMP: is_thread_compiled_alt PO PI),
-      mm_similar_states_alt (init PO) (init PI).
-  Proof.
-    (* should shorten it a lot *)
-    ins. red. simpl. splits; auto.
-    { apply compiled_empty_alt. }
-    assert (NO_E: E init_execution ≡₁ ∅) by basic_solver. 
-    assert (PREPEND_E0: forall S i (IN_E: S ⊆₁ E init_execution), prepend_events S i ≡₁ ∅).
-    { intros. split; [| basic_solver].
-      red. intros e.
-      intros PREP.
-      do 2 red in PREP. apply IN_E in PREP.
-      unfold acts_set in PREP. simpl in PREP. auto. }
-    assert (PREPEND_EAPP: forall S i x (IN_E: S ⊆₁ E init_execution), prepend_events S i x -> False).
-    { intros. specialize (PREPEND_E0 S i IN_E). red in PREPEND_E0. desc.
-      red in PREPEND_E0. specialize (PREPEND_E0 x H). basic_solver. }      
-    red.
-    splits. 
-    { rewrite PREPEND_E0; [| basic_solver]. rewrite PREPEND_E0; [| basic_solver].
-      rewrite PREPEND_E0; [| basic_solver]. basic_solver. }
-    { auto. }
-    { intros. exfalso. apply (PREPEND_EAPP ((E init_execution ∩₁ Sc init_execution)) 2 e); [basic_solver | auto]. }
-    { intros. exfalso. apply (PREPEND_EAPP ((E init_execution ∩₁ W init_execution ∩₁ ORlx init_execution)) 2 e); [basic_solver | auto]. }
-    { intros. exfalso. apply (PREPEND_EAPP (E init_execution ∩₁ W init_execution ∩₁ Sc init_execution) 1 e);  [basic_solver | auto]. }
-    simpl. split; [basic_solver|].
-    red. intros. desc. red in H. desc. red in H. desc. basic_solver. 
-  Qed.
-
-  Lemma thread_execs tid PO PI (COMP: is_thread_compiled_alt PO PI)
-        SGI (ExI: thread_execution tid PI SGI):
-    exists SGO, Othread_execution tid PO SGO /\
-           same_behavior_local SGO SGI /\
-           Wf_local SGO. 
-  Proof.
-    intros.
-    destruct ExI as [sti EXECI]. desc.
-    set (lenO := length PO). set (lenI := length PI).
-    assert (STI_INSTRS: instrs sti = PI) by admit. 
-    assert (OSEQ_STEPS: (oseq_step tid)＊ (init PI) sti). 
-    { admit. }
-    
-    apply crt_num_steps in OSEQ_STEPS as [oseq_num OSEQ_REACH]. 
-    assert (STO_SEQ: forall k sti_k (INDEX: k <= oseq_num)
-                       (CUR_STEPS: (oseq_step tid) ^^ k (init PI) sti_k),
-               exists sto_k, (Ostep tid) ^^ k (init PO) sto_k
-                        /\ mm_similar_states_alt sto_k sti_k).
-    { intros k.
-      induction k.
-      { exists (init PO). split.
-        - basic_solver.
-        - do 2 red in CUR_STEPS. desc. rewrite <- CUR_STEPS.
-          apply init_mm_same; auto. }
-      intros. 
-      apply step_prev in CUR_STEPS as [sti_cur [OSEQ_REACH_CUR OSEQ_NEXT]].
-      forward eapply (IHk sti_cur).
-      { omega. }
-      { auto. }
-      intros [sto_cur [OSTEP_REACH_CUR MM_SIM_CUR]].
-      pose proof (pair_step_alt MM_SIM_CUR OSEQ_NEXT) as [sto_next [OSTEP_NEXT MM_SIM_NEXT]].
-      exists sto_next. split; auto.
-      apply step_prev. exists sto_cur. split; auto. } 
-    
-    destruct (@STO_SEQ oseq_num sti (Nat.le_refl oseq_num) OSEQ_REACH) as [sto [osteps_num MM_SIM]].
-    exists (G sto).
-    splits.
-    3: { (* Wf_local for derived sto graph *) admit. }
-    2: { red in MM_SIM. desc. vauto. }
-    red. exists sto. splits; auto. 
-    { apply crt_num_steps. basic_solver 10. }
-    red.
-    (* why pc should be strictly larger than l? *) admit.
-  Admitted. 
-
-  Lemma PREP_NOT_LAST' e sto (PREPS: exists S i, prepend_events S i e /\ S ⊆₁ E (G sto)) (EXISTING_INDICES: forall e', E (G sto) e' -> index e' < eindex sto):
-    index e <> eindex sto.
-  Proof. 
-    intros INDEQ. 
-    destruct PREPS as [S [i [PREPS INE]]].
-    do 2 red in PREPS. 
-    specialize (INE (ThreadEvent (tid e) (index e + i)) PREPS).
-    apply EXISTING_INDICES in INE.
-    simpl in INE.
-    omega.
-  Qed.    
-    
-  Lemma restricted_wf GI SGI tid (WF: Wf GI) (TRI: thread_restricted_execution GI tid SGI): Wf SGI. 
-  Proof.
-  Admitted.
-        
-  Lemma wf_split G: Wf G <-> Wf_global G /\ (forall tid SG (TRE: thread_restricted_execution G tid SG), Wf_local SG). 
-  Proof.
-    (* destruct WFG. split; auto. *)
-    (* { ins. desc. set (t := tid a). *)
-    (*   specialize (WFL t). *)
-    (*   admit. } *)
-  Admitted.
-
-  Lemma tre_idempotent SG tid G (TRE: thread_restricted_execution G tid SG):
-    thread_restricted_execution SG tid SG.
-  Proof. Admitted.
-
-
-  Lemma Wf_subgraph G' G (SB: same_behavior G G') (WF: Wf G'): Wf G.
-  Proof.
-    (* split. *)
-    (* red in SB. desc. red in SAME_LOCAL. desc.  *)
-  Admitted.
-      
-End OCamlMM_TO_IMM_S_PROG.
-  
-
-Section CompilationCorrectness.
-
-  Notation "'E' G" := G.(acts_set) (at level 1).
-  Notation "'R' G" := (fun a => is_true (is_r G.(lab) a)) (at level 1).
-  Notation "'W' G" := (fun a => is_true (is_w G.(lab) a)) (at level 1).
-  Notation "'RW' G" := (R G ∪₁ W G) (at level 1).
-  Notation "'F' G" := (fun a => is_true (is_f G.(lab) a)) (at level 1).
-  Notation "'ORlx' G" := (fun a => is_true (is_only_rlx G.(lab) a)) (at level 1).
-  Notation "'Sc' G" := (fun a => is_true (is_sc G.(lab) a)) (at level 1). 
-  Notation "'Acq' G" := (fun a => is_true (is_acq G.(lab) a)) (at level 1). 
-  Notation "'Acqrel' G" := (fun a => is_true (is_acqrel G.(lab) a)) (at level 1). 
-  Notation "'R_ex' G" := (fun a => is_true (R_ex G.(lab) a)) (at level 1).
-  Notation "'hbo'" := (OCaml.hb). 
-  Notation "'same_loc' G" := (same_loc G.(lab)) (at level 1).
-  Notation "'Tid_' t" := (fun x => tid x = t) (at level 1).
-  Variable ProgO ProgI: Prog.Prog.t.
-  Hypothesis Compiled: is_compiled ProgO ProgI.
-  Hypothesis OCamlProgO: OCamlProgram ProgO.
-  
-  Variable GI: execution.
-  Hypothesis WFI: Wf GI.
-  Variable sc: relation actid. 
-  Hypothesis ExecI: program_execution ProgI GI.
-  Hypothesis IPC: imm_s.imm_psc_consistent GI sc.
-
-  Definition merge_thread_graphs (graphs: list (thread_id * execution)) : execution.
-  Admitted. 
-
-  Lemma GO_exists: exists GO,
-      Oprogram_execution OCamlProgO GO /\
-      same_behavior GO GI. 
-  Proof.
-    pose proof thread_execs.
-    assert (ALL_SGO: forall tid PO PI SGI
-                       (THREADO: IdentMap.find tid ProgO = Some PO)
-                       (THREADI: IdentMap.find tid ProgI = Some PI)
-                       (THREAD_EXEC: thread_execution tid PI SGI),
-                 exists SGO, Othread_execution tid PO SGO /\
-                        same_behavior_local SGO SGI /\ Wf_local SGO). 
-    { admit. }
-    (* should somehow get a list of threads and call merge_thread_graphs *)
-    (* also should pass rf and co to resulting graph *)
-    assert (exists GO, forall tid PO PI SGI
-                    (THREADO: IdentMap.find tid ProgO = Some PO)
-                    (THREADI: IdentMap.find tid ProgI = Some PI)
-                    (THREAD_EXEC: thread_execution tid PI SGI),
-                 exists SGO, Othread_execution tid PO SGO /\
-                        same_behavior_local SGO SGI /\ Wf_local SGO /\
-                        thread_restricted_execution GO tid SGO) as [GO SUBGRAPHS]. 
-    { admit. }
-    exists GO.
-    split.
-    { red. split.
-      { admit. }
-      (* red in ExecI. destruct ExecI. specialize (H1 tid  *)
-      (* intros tid PO THREADO. specialize (SUBGRAPHS tid PO).  *)
-      admit. 
-    } 
-    red.
-    splits.
-    { (* should show that if every thread graph is sbl, then the whole graph is sbl*)
-      admit. }
-    { admit. }
-    admit.     
-  Admitted.
-
-  Lemma graph_switch GO (SB: same_behavior GO GI) (OMM_I: ocaml_consistent GI):
-    ocaml_consistent GO.
-  Proof.
-    assert (E': E GO ≡₁ E GI ∩₁ (RW GI \₁ dom_rel (GI.(rmw)))).
-    { admit. }
-    red in SB. desc. 
-    assert (RF': rf GO ≡ rf GI ⨾ ⦗set_compl (dom_rel (rmw GI))⦘).
-    { rewrite EXT_RF. basic_solver. }
-    assert (SB': sb GO ≡ ⦗RW GI \₁ dom_rel (rmw GI)⦘ ⨾ sb GI ⨾ ⦗RW GI \₁ dom_rel (rmw GI)⦘).
-    { unfold Execution.sb.        
-      rewrite !seqA. do 2 seq_rewrite <- id_inter.
-      rewrite set_interC. 
-      rewrite E'. 
-      basic_solver. }
-    assert (LAB': GO.(lab) = GI.(lab)).
-    { red in SAME_LOCAL. desc. auto. }
-    assert (SC': Sc GO ≡₁ Sc GI). 
-    { rewrite LAB'. auto. }
-    assert (HBO': hbo GO ⊆ hbo GI).
-    { unfold OCaml.hb. rewrite SC'. apply clos_trans_mori.
-      apply union_mori; [rewrite SB'; basic_solver | ].
-      hahn_frame. 
-      apply union_mori; [rewrite SAME_CO; basic_solver | rewrite RF'; basic_solver]. }
-    assert (CO': co GO ≡ co GI) by intuition.
-    assert (FR': fr GO ≡ ⦗set_compl (dom_rel (rmw GI))⦘ ⨾ fr GI).
-    { unfold fr. rewrite CO'. rewrite <- seqA. apply seq_more; [| basic_solver].
-      rewrite RF'.  basic_solver. }
-    red. red in OMM_I.
-    splits; auto.
-    { red. rewrite E', RF'.
-      desc. red in Comp.
-      rewrite set_interC, <- set_interA.
-      rewrite set_inter_minus_r.
-      arewrite (R GO ∩₁ E GI ∩₁ RW GI ≡₁ R GO ∩₁ E GI) by rewrite LAB'; basic_solver.
-      rewrite codom_eqv1.
-      rewrite set_minusE.
-      apply set_subset_inter.
-      { rewrite set_interC. rewrite LAB'. apply Comp. }
-      basic_solver. }
-    { assert (NO_RMW: rmw GO ≡ ∅₂) by admit. 
-      red. rewrite NO_RMW. basic_solver. }
-    { rewrite HBO', CO'. desc.  auto. }
-    { unfold fr. rewrite HBO', CO'. 
-      arewrite (rf GO ⊆ rf GI) by rewrite RF'; auto. 
-      auto. desc. auto. }    
-    assert (W_RMW: W GI ⊆₁ RW GI \₁ dom_rel (rmw GI)).
-    { rewrite set_minusE.
-      apply set_subset_inter_r. split; [basic_solver| ].
-      rewrite (WFI.(wf_rmwD)).
-      rewrite dom_eqv1. rewrite set_compl_inter.
-      unionR left. type_solver. }
-    arewrite (rfe GO ⊆ rfe GI).
-    { unfold rfe. rewrite SB', RF'.
-      apply inclusion_minus_l.
-      rewrite rfi_union_rfe at 1. rewrite seq_union_l.
-      apply union_mori.        
-      { rewrite (WFI.(wf_rfiD)). 
-        arewrite (rfi GI ⊆ sb GI).
-        apply seq_mori; [ | basic_solver]. 
-        apply eqv_rel_mori. apply W_RMW. }
-      unfold rfe. basic_solver. }
-    arewrite (fre GO ⊆ fre GI).
-    { unfold fre. rewrite SB', FR'.
-      apply inclusion_minus_l.
-      rewrite fri_union_fre at 1. rewrite seq_union_r.
-      apply union_mori.        
-      { rewrite (WFI.(wf_friD)). 
-        arewrite (fri GI ⊆ sb GI).
-        rewrite <- seqA. 
-        apply seq_mori; [basic_solver |].
-        hahn_frame. apply eqv_rel_mori. apply W_RMW. }
-      unfold fre. basic_solver. }
-    
-    arewrite (coe GO ⊆ coe GI).
-    { unfold coe. rewrite SB', CO'. 
-      apply inclusion_minus_l.
-      rewrite coi_union_coe at 1. 
-      apply union_mori.        
-      { rewrite (WFI.(wf_coiD)). 
-        arewrite (coi GI ⊆ sb GI).
-        apply seq_mori; hahn_frame; apply eqv_rel_mori; apply W_RMW. } 
-      unfold coe. basic_solver. }
-    rewrite SC'. 
-    arewrite (sb GO ⊆ sb GI) by rewrite SB'; basic_solver.
-    desc. auto.
-  Admitted.
-  
-  Lemma imm_implies_omm GO (WFO: Wf GO) (SB: same_behavior GO GI):
-    ocaml_consistent GI.
-  Proof.
-    red in SB. desc.
-    forward eapply (@OCamlToimm_s.imm_to_ocaml_consistent GI).
-    { admit. }
-    { admit. }
-    { admit. }
-    { admit. }
-    { admit. }
-    { auto. }
-    { eauto. }
-    auto. 
-  Admitted. 
-  
-  Theorem compilation_correctness: exists (GO: execution),
-      ⟪WFO: Wf GO ⟫ /\
-      ⟪ExecO: Oprogram_execution OCamlProgO GO⟫ /\
-      ⟪OC: ocaml_consistent GO ⟫ /\
-      ⟪SameBeh: same_behavior GO GI⟫.
-  Proof.
-    pose proof GO_exists as [GO [OPE EVENTS]].
-    exists GO.
-    pose proof (Wf_subgraph EVENTS WFI) as WFO. 
-    splits; auto.
-    apply graph_switch; auto.
-    apply (imm_implies_omm WFO); auto.
-  Qed. 
-
-End CompilationCorrectness.       
