src/ocamlmm/OCamlToimm_s_prog_compilation.v
@@ -1,0 +1,103 @@
+From hahn Require Import Hahn.
+Require Import Omega.
+Require Import Events.
+Require Import Execution.
+Require Import Execution_eco.
+Require Import imm_common.
+Require Import imm_s_hb.
+Require Import imm_s.
+Require Import OCamlToimm_s_prog. 
+Require Import ClosuresProperties. 
+Require Import Prog.
+Require Import ProgToExecution.
+Require Import ProgToExecutionProperties.
+From PromisingLib Require Import Basic Loc.
+Require Import Basics. 
+Set Implicit Arguments.
+
+
+Section OCaml_IMM_Compilation.   
+
+  Definition exchange_reg: Reg.t.
+    vauto.
+  Admitted.      
+
+  Inductive is_instruction_compiled: Prog.Instr.t -> list Prog.Instr.t -> Prop :=
+  | compiled_Rna lhs loc:
+      let ld := (Instr.load Orlx lhs loc) in
+      is_instruction_compiled (ld) ([ld])
+  | compiled_Wna loc val:
+      let st := (Instr.store Orlx loc val) in
+      let f := (Instr.fence Oacqrel) in
+      is_instruction_compiled (st) ([f; st])
+  | compiled_Rat lhs loc:
+      let ld := (Instr.load Osc lhs loc) in
+      let f := (Instr.fence Oacq) in
+      is_instruction_compiled (ld) ([f; ld])
+  | compiled_Wat loc val:
+      let st := (Instr.store Osc loc val) in
+      let exc := (Instr.update (Instr.exchange val) Xpln Osc Osc exchange_reg loc) in
+      let f := (Instr.fence Oacq) in
+      is_instruction_compiled (st) ([f; exc])
+  | compiled_assign lhs rhs:
+      let asn := (Instr.assign lhs rhs) in
+      is_instruction_compiled (asn) ([asn])
+  | compiled_ifgoto e n:
+      let igt := (Instr.ifgoto e n) in
+      is_instruction_compiled (igt) ([igt]).
+
+  Definition is_thread_block_compiled PO BPI := Forall2 is_instruction_compiled PO BPI. 
+
+  Definition is_thread_compiled PO PI :=
+    exists BPI, is_thread_block_compiled PO BPI /\ PI = flatten BPI. 
+      
+  Definition is_compiled (po: Prog.Prog.t) (pi: Prog.Prog.t) :=
+    ⟪ SAME_THREADS: forall t_id, IdentMap.In t_id po <-> IdentMap.In t_id pi ⟫ /\
+    ⟪ THREADS_COMPILED: forall thread to ti (TO: Some to = IdentMap.find thread po)
+      (TI: Some ti = IdentMap.find thread pi), is_thread_compiled to ti ⟫. 
+
+  Lemma every_instruction_compiled PO BPI (COMP: is_thread_block_compiled PO BPI)
+        i instr block (INSTR: Some instr = nth_error PO i)
+        (BLOCK: Some block = nth_error BPI i):
+    is_instruction_compiled instr block.
+  Proof.
+    generalize dependent BPI. generalize dependent i.
+    generalize dependent instr. generalize dependent block. 
+    induction PO.
+    - ins.
+      assert (forall {A: Type}, nth_error ([]: list A) i = None). 
+      { ins. apply nth_error_None. simpl. omega. }
+      rewrite H in INSTR. vauto.
+    - ins. inversion COMP. subst.
+      destruct (NPeano.Nat.zero_or_succ i).
+      + subst. simpl in *. congruence.
+      + desc. subst. simpl in *. 
+        apply (@IHPO block instr m INSTR l' H3 BLOCK). 
+  Qed. 
+
+  Lemma compilation_same_length PO BPI (COMP: is_thread_block_compiled PO BPI):
+    length PO = length BPI.
+  Proof.
+    generalize dependent BPI.
+    induction PO.
+    { ins. inversion COMP. auto. }
+    ins. inversion COMP. simpl.
+    intuition.
+  Qed. 
+
+  Lemma steps_same_instrs sti sti' (STEPS: exists tid, (step tid)＊ sti sti'):
+    instrs sti = instrs sti'.
+  Proof.
+    destruct STEPS as [tid STEPS]. apply crt_num_steps in STEPS.
+    destruct STEPS as [n STEPS].
+    generalize dependent sti'.
+    induction n.
+    - intros sti' STEPS. simpl in STEPS. generalize STEPS. basic_solver 10.
+    - intros sti' STEPS.
+      rewrite step_prev in STEPS. destruct STEPS as [sti'' STEPS'']. desc.
+      replace (instrs sti) with (instrs sti'').
+      { red in STEPS''0. desf. red in STEPS''0. desf. }
+      symmetry. eapply IHn. eauto.
+  Qed.
+
+End OCaml_IMM_Compilation.   
